Simplify LL(1) derivation relation, add a parser soundness proof w.r.t. this relation

LL1/LL1_Derivation.v
@@ -6,6 +6,7 @@ Open Scope list_scope.
 
 (* "symbol Sym derives input prefix Pre, producing tree Tr
     and leaving input suffix Suf unconsumed" *)
+(*
 Inductive sym_derives_prefix {g : grammar} :
   symbol -> list string -> tree -> list string -> Prop :=
 | T_sdp : 
@@ -49,6 +50,37 @@ with gamma_derives_prefix {g : grammar} :
                                         (Fcons hdTree tlTrees)
                                         (wpre ++ wmid)
             *)
+            *)
+
+Inductive sym_derives_prefix {g : grammar} :
+  symbol -> list string -> tree -> list string -> Prop :=
+| T_sdp : 
+    forall (y : string) (rem : list string),
+      sym_derives_prefix (T y) [y] (Leaf y) rem
+| NT_sdp :
+    forall (x : string) 
+           (gamma : list symbol)
+           (word rem : list string) 
+           (subtrees : forest),
+      (@isLookaheadFor g) (peek (word ++ rem)) (NT x) gamma
+      -> gamma_derives_prefix gamma word subtrees rem
+      -> sym_derives_prefix (NT x) word (Node x subtrees) rem
+with gamma_derives_prefix {g : grammar} : 
+       list symbol -> list string -> forest -> list string -> Prop :=
+     | Nil_gdp : forall rem,
+         gamma_derives_prefix [] [] Fnil rem
+     | Cons_gdp : 
+         forall (hdRoot : symbol)
+                (wpre wsuf rem : list string)
+                (hdTree : tree)
+                (tlRoots : list symbol)
+                (tlTrees : forest),
+         sym_derives_prefix hdRoot wpre hdTree (wsuf ++ rem)
+         -> gamma_derives_prefix tlRoots wsuf tlTrees rem
+         -> gamma_derives_prefix (hdRoot :: tlRoots) 
+                                 (wpre ++ wsuf)
+                                 (Fcons hdTree tlTrees)
+                                 rem.
 
 Scheme sdp_mutual_ind :=
   Induction for sym_derives_prefix Sort Prop
@@ -206,6 +238,18 @@ Proof.
     + auto.
 Qed.
 
+Lemma lookahead_in_grammar :
+  forall g la x gamma,
+    (@isLookaheadFor g) la (NT x) gamma
+    -> In (x, gamma) (productions g).
+Proof.
+  intros.
+  destruct H as [Hfi | Hfo].
+  - inv Hfi; auto.
+  - destruct Hfo.
+    inv H; auto.
+Qed.
+
 Lemma gamma_derives_nil_nullable :
   forall g gamma wpre f wsuf,
     (@gamma_derives_prefix g) gamma wpre f wsuf
@@ -224,11 +268,11 @@ Proof.
                wpre = nil
                -> nullableGamma gamma); intros; subst.
   - inv H.
-  - inv f; simpl in *.
-    eapply eof_fgamma in H2; eauto; inv H2.
-  - inv f.
-    econstructor.
+(*  - inv f; simpl in *.
+    eapply eof_fgamma in H2; eauto; inv H2. *)
+  - econstructor.
     econstructor; eauto.
+    apply lookahead_in_grammar in i; auto.
   - constructor.
   - apply app_eq_nil in H; destruct H; subst.
     destruct hdRoot as [y | x].
@@ -236,6 +280,152 @@ Proof.
     + econstructor; eauto.
 Qed.
 
+Lemma gamma_derives_cons_fg :
+  forall g gamma word f rem,
+    (@gamma_derives_prefix g) gamma word f rem
+    -> forall tok toks,
+      word = tok :: toks
+      -> (@firstGamma g) (LA tok) gamma.
+Proof.
+  intros g gamma word f rem Hder.
+  induction Hder using gdp_mutual_ind with
+      (P := fun sym word tr rem
+                (pf : sym_derives_prefix sym word tr rem) =>
+              forall tok toks,
+                word = tok :: toks
+                -> firstSym (LA tok) sym)
+      (P0 := fun gamma word f rem
+                 (pf : gamma_derives_prefix gamma word f rem)
+             =>
+               forall tok toks,
+                 word = tok :: toks
+                 -> firstGamma (LA tok) gamma); intros; subst.
+  - inv H; constructor.
+  - simpl in *.
+    apply lookahead_in_grammar in i.
+    econstructor.
+    econstructor; eauto.
+  - inv H.
+  - destruct hdRoot.
+    + inv s.
+      inv H.
+      constructor.
+      constructor.
+    + destruct wpre as [| ptok ptoks]; simpl in *.
+      * eapply FiGammaTl.
+        -- inv s; simpl in *.
+           apply lookahead_in_grammar in H1.
+           econstructor.
+           econstructor; eauto.
+           eapply gamma_derives_nil_nullable; eauto.
+        -- eapply IHHder0; eauto.
+      * inv H.
+        eapply FiGammaHd.
+        eapply IHHder; eauto.
+Qed.
+        
+Lemma der_det :
+  forall tbl g,
+    isParseTableFor tbl g
+    -> forall sym word rem tr,
+      (@sym_derives_prefix g) sym word tr rem
+      -> forall word' rem' tr',
+        (@sym_derives_prefix g) sym word' tr' rem'
+        -> word ++ rem = word' ++ rem'
+        -> word = word' /\ rem = rem' /\ tr = tr'.
+Proof.
+  intros tbl g Htbl sym word rem tr Hder.
+  induction Hder using sdp_mutual_ind with
+      (P := fun sym word tr rem
+                (pf : sym_derives_prefix
+                        sym word tr rem) =>
+              forall word' rem' tr',
+                sym_derives_prefix sym word' tr' rem'
+                -> word ++ rem = word' ++ rem'
+                -> word = word' /\ rem = rem' /\ tr = tr')
+      (P0 := fun gamma word f rem
+                 (pf : gamma_derives_prefix gamma word f rem) =>
+               forall word' rem' f',
+                 gamma_derives_prefix gamma word' f' rem'
+                 -> word ++ rem = word' ++ rem'              
+                 -> word = word' /\ rem = rem' /\ f = f'); intros.
+  - inv H; inv H0; auto.
+    
+  - (* Nt case *)
+    inv H.
+    assert (gamma0 = gamma).
+    { destruct i as [Hfi | Hfo].
+      - destruct H2 as [Hfi' | Hfo'].
+        + rewrite <- H0 in Hfi'.
+          destruct Htbl as [Hmin Hcom].
+          unfold ptComplete in Hcom.
+          assert ((@isLookaheadFor g) (peek (word ++ rem))
+                                       (NT x)
+                                       gamma).
+           { left; auto. }
+           assert ((@isLookaheadFor g) (peek (word ++ rem))
+                                       (NT x)
+                                       gamma0).
+           { left; auto. }
+           apply Hcom in H.
+           apply Hcom in H1.
+           destruct H as [m [Hs Hl]].
+           destruct H1 as [m' [Hs' Hl']].
+           congruence.
+        + exfalso.
+          destruct Hfo'.
+          eapply no_first_follow_conflicts with (sym := NT x); eauto.
+          * econstructor; eauto.
+          * econstructor; eauto.
+          * inv H1.
+            rewrite H0.
+            auto.
+      - destruct H2 as [Hfi' | Hfo'].
+        + exfalso.
+          destruct Hfo.
+          eapply no_first_follow_conflicts with (sym := NT x); eauto.
+           * econstructor; eauto.
+           * econstructor; eauto.
+           * inv H1.
+             rewrite <- H0.
+             auto.
+        + destruct Hfo; destruct Hfo'.
+          destruct Htbl as [Hmin Hcom].
+          unfold ptComplete in Hcom.
+          rewrite <- H0 in H4.
+          assert ((@isLookaheadFor g) (peek (word ++ rem))
+                                       (NT x)
+                                       gamma).
+          { right; split; auto. }
+           assert ((@isLookaheadFor g) (peek (word ++ rem))
+                                       (NT x)
+                                       gamma0).
+          { right; split; auto. }
+          apply Hcom in H5.
+          apply Hcom in H6.
+          destruct H5 as [m [Hs Hl]].
+          destruct H6 as [m' [Hs' Hl']].
+          congruence. }
+    subst.
+    eapply IHHder in H3; eauto.
+    destruct H3.
+    destruct H1.
+    subst; auto.
+
+  - inv H; auto.
+
+  - inv H.
+    eapply IHHder in H3; eauto.
+    + destruct H3.
+      destruct H1; subst.
+      eapply IHHder0 in H7; eauto.
+      destruct H7.
+      destruct H2.
+      subst; auto.
+    + repeat rewrite app_assoc; auto.
+Qed. 
+
+(*
 Lemma der_det :
   forall tbl g,
     isParseTableFor tbl g
@@ -377,6 +567,7 @@ Proof.
       destruct H2.
       subst; auto.
     + repeat rewrite app_assoc; auto.
-Qed. (* Finally! *)            
-
+Qed.
+ *)
+(* This is an older, not as clean version of the relation *)
     
