LL1/LL1_Soundness.v
@@ -1,0 +1,207 @@
+Require Import List Omega String.
+Require Import ExampleGrammars Grammar
+               Lemmas LL1.Parser Lib.Tactics ParseTable
+               ParseTree Lib.Utils LL1.LL1_Derivation.
+Import ListNotations.
+Open Scope list_scope.
+
+Lemma beqString_eq : 
+  forall s s2,
+    beqString s s2 = true
+    -> s = s2.
+Proof.
+  intros; unfold beqString in H.
+  destruct (StringMapFacts.eq_dec s s2); trivial.
+  inv H.
+Qed.
+
+Lemma parse_t_ret_leaf :
+  forall tbl y input fuel tree suffix,
+    parse tbl (T y) input fuel = (Some tree, suffix) ->
+    isLeaf tree = true.
+Proof.
+  intros. destruct fuel.
+  - inv H.
+  - simpl in H. destruct input.
+    + inv H.
+    + destruct (Utils.beqString y s).
+      * inv H. reflexivity.
+      * inv H.
+Qed.
+
+Lemma parse_nt_ret_node :
+  forall tbl x input fuel tree suffix,
+    parse tbl (NT x) input fuel = (Some tree, suffix)
+    -> isNode tree = true.
+Proof.
+  intros. destruct fuel.
+  - simpl in H. inv H.
+  - simpl in H. destruct (parseTableLookup x (peek input) tbl).
+    + destruct (parseForest tbl l input fuel). 
+      destruct o. 
+      * inv H. trivial.
+      * inv H.
+    + inv H. 
+Qed.
+
+Lemma tbl_entry_is_lookahead :
+  forall tbl g x la gamma,
+    isParseTableFor tbl g
+    -> parseTableLookup x la tbl = Some gamma
+    -> (@isLookaheadFor g) la (NT x) gamma.
+Proof.
+  intros tbl g x la gamma Htbl Hlkp.
+  destruct Htbl as [Hmin Hcom].
+  unfold ptMinimal in Hmin.
+  unfold parseTableLookup in Hlkp.
+  destruct (StringMap.find x tbl) as [m |] eqn:Hsf.
+  - eapply Hmin; eauto.
+  - inv Hlkp.
+Qed.
+
+Theorem parse_correct :
+  forall (g   : grammar)
+         (tbl : parse_table),
+    isParseTableFor tbl g
+    -> forall (tr        : tree)
+              (sym       : symbol)
+              (input rem : list string)
+              (fuel      : nat),
+      parse tbl sym input fuel = (Some tr, rem)
+      -> exists word,
+        word ++ rem = input
+        /\ (@sym_derives_prefix g) sym word tr rem.
+Proof.
+  intros g tbl Htbl tr. 
+  induction tr as [ s
+                  | s f IHpf
+                  |
+                  | tr IHp f IHpf ]
+                    using tree_mutual_ind with
+      
+      (P := fun tr =>
+              forall sym input rem fuel,
+                parse tbl sym input fuel =
+                (Some tr, rem)
+                -> exists word,
+                  word ++ rem = input
+                  /\ sym_derives_prefix sym word tr rem)
+      
+      (P0 := fun f =>
+               forall gamma input rem fuel,
+                 parseForest tbl gamma input fuel =
+                 (Some f, rem)
+                 -> exists word,
+                   word ++ rem = input
+                   /\ gamma_derives_prefix gamma word f rem).
+
+  - (* T case *)
+    intros sym input rem fuel Hp.
+    destruct fuel as [| fuel].
+    + inv Hp.
+    + destruct sym as [y | x].
+      * destruct input as [| tok toks]; simpl in *.
+        -- inv Hp.
+        -- destruct (beqString y tok) eqn:Hbeq.
+           ++ inv Hp.
+              exists [tok]; split; auto.
+              apply beqString_eq in Hbeq.
+              rewrite Hbeq; constructor.
+           ++ inv Hp.
+      * apply parse_nt_ret_node in Hp; inv Hp.
+
+  - (* NT case *)
+    intros sym input rem fuel Hp.
+    destruct fuel as [| fuel].
+    + inv Hp.
+    + destruct sym as [y | x].
+      * apply parse_t_ret_leaf in Hp; inv Hp.
+      * simpl in Hp. 
+        destruct (parseTableLookup x (peek input) tbl)
+          as [ys |] eqn:Hlkp.
+        -- destruct (parseForest tbl ys input fuel)
+            as [subres input'] eqn:Hpf.
+           destruct subres as [subtrees |].
+           ++ inv Hp.
+              apply IHpf in Hpf; clear IHpf.
+              destruct Hpf as [word].
+              destruct H.
+              exists word.
+              split; auto.
+              eapply tbl_entry_is_lookahead in Hlkp; eauto.
+              econstructor; eauto.
+              rewrite H.
+              auto.
+           ++ inv Hp.
+        -- inv Hp.
+
+  - (* Fnil case *)
+    intros gamma input rem fuel Hpf.
+    destruct fuel as [| fuel].
+    + inv Hpf.
+    + destruct gamma as [| hdSym tlSyms].
+      * simpl in Hpf.
+        inv Hpf.
+        exists nil; simpl.
+        split; auto.
+        constructor.
+      * exfalso.
+        simpl in Hpf.
+        destruct (parse tbl hdSym input fuel)
+          as [subres input'].
+        destruct subres as [lSib |].
+        -- destruct (parseForest tbl tlSyms input' fuel)
+            as [subres input''].
+           destruct subres as [rSibs |]; inv Hpf.
+        -- inv Hpf.
+
+  - (* Fcons case *)
+    intros gamma input rem fuel Hpf.
+    destruct fuel as [| fuel].
+    + inv Hpf.
+    + destruct gamma as [| hdSym tlSyms]; simpl in Hpf.
+      * inv Hpf.
+      * destruct (parse tbl hdSym input fuel) as
+            [subres input'] eqn:Hp.
+        destruct subres as [lSib |].
+        -- destruct (parseForest tbl tlSyms input' fuel) as
+              [subres input''] eqn:Hpf'.
+           destruct subres as [rSibs |].
+           ++ inv Hpf.
+              eapply IHp in Hp.
+              destruct Hp as [wpre [Happ Hder]].
+              apply IHpf in Hpf'.
+              destruct Hpf' as [wsuf [Happ' Hder']].
+              exists (wpre ++ wsuf).
+              split.
+              ** rewrite <- Happ.
+                 rewrite <- Happ'.
+                 rewrite app_assoc.
+                 auto.
+              ** econstructor; eauto.
+                 rewrite Happ'.
+                 auto.
+           ++ inv Hpf.
+        -- inv Hpf.
+Qed.
+
+(* This version specifies exactly what prefix of the input
+   is consumed *)
+Corollary parse_correct' :
+  forall (g   : grammar)
+         (tbl : parse_table),
+    isParseTableFor tbl g
+    -> forall (tr       : tree)
+              (sym      : symbol)
+              (word rem : list string)
+              (fuel     : nat),
+      parse tbl sym (word ++ rem) fuel = (Some tr, rem)
+      -> (@sym_derives_prefix g) sym word tr rem.
+Proof.
+  intros g tbl Htbl tr sym word rem fuel Hp.
+  pose proof Hp as Hp'.
+  eapply parse_correct in Hp; eauto.
+  destruct Hp as [word' [Happ Hder]].
+  apply app_inv_tail in Happ.
+  subst; auto.
+Qed.
